Weakening and substitution WIP

theories/Induction.v
@@ -1,11 +1,25 @@
 Require Import List Program.
 Require Import Template.Template Template.Ast.
 Require Import BinPos.
-Require Import Coq.Arith.Compare_dec.
+Require Import Coq.Arith.Compare_dec Bool.
 Set Asymmetric Patterns.
+
+Arguments dname {term} _.
+Arguments dtype {term} _.
+Arguments dbody {term} _.
+Arguments rarg {term} _.
 
 Definition on_snd {A B} (f : B -> B) (p : A * B) :=
   (fst p, f (snd p)).
+
+Definition map_def {term : Set} (f : term -> term) (d : def term) :=
+  {| dname := d.(dname); dtype := f d.(dtype); dbody := f d.(dbody); rarg := d.(rarg) |}.
+
+Definition test_snd {A B} (f : B -> bool) (p : A * B) :=
+  f (snd p).
+
+Definition test_def {term : Set} (f : term -> bool) (d : def term) :=
+  f d.(dtype) && f d.(dbody).
 
 Lemma on_snd_on_snd {A B} (f g : B -> B) (d : A * B) :
   on_snd f (on_snd g d) = on_snd (fun x => f (g x)) d.
@@ -19,8 +33,6 @@ Proof.
   reflexivity.
 Qed.
 
-Definition map_def {term : Set} (f : term -> term) (d : def term) :=
-  {| dname := d.(dname _); dtype := f d.(dtype _); dbody := f d.(dbody _); rarg := d.(rarg _) |}.
 
 Lemma map_def_map_def {term : Set} (f g : term -> term) (d : def term) :
   map_def f (map_def g d) = map_def (fun x => f (g x)) d.
@@ -53,13 +65,17 @@ Proof.
   rewrite H. f_equal. eauto.
 Qed.
 
+Lemma map_def_id {t : Set} : map_def (@id t) = id.
+Proof. extensionality p. now destruct p. Qed.
+Hint Rewrite @map_def_id @map_id.
+
 (** Custom induction principle on syntax, dealing with the various lists appearing in terms. *)
 
 Definition tCaseBrsProp (P : term -> Prop) (P0 : list term -> Prop) (l : list (nat * term)) :=
   Forall (fun x => P (snd x)) l.
 
 Definition tFixProp (P : term -> Prop) (P0 : list term -> Prop) (m : mfixpoint term) :=
-  Forall (fun x : def term => P x.(dtype _) /\ P x.(dbody _)) m.
+  Forall (fun x : def term => P x.(dtype) /\ P x.(dbody)) m.
 
 Lemma term_ind_list :
   forall P0 : list term -> Prop,
@@ -160,7 +176,7 @@ Proof.
 Qed.
 
 Lemma map_def_spec (P : term -> Prop) (f g : term -> term) (x : def term) :
-  P x.(dbody _) -> P x.(dtype _) -> (forall x, P x -> f x = g x) ->
+  P x.(dbody) -> P x.(dtype) -> (forall x, P x -> f x = g x) ->
   map_def f x = map_def g x.
 Proof.
   intros. destruct x. unfold map_def. simpl.
@@ -187,12 +203,73 @@ Proof.
   eapply map_def_spec; eauto.
 Qed.
 
+
+Lemma forall_forallb_map_spec {A : Type} {P : A -> Prop} {p : A -> bool}
+      {l : list A} {f g : A -> A} :
+    Forall P l -> forallb p l = true ->
+    (forall x : A, P x -> p x = true -> f x = g x) -> map f l = map g l.
+Proof.
+  induction 1; simpl; trivial.
+  rewrite andb_true_iff. intros [px pl] Hx.
+  f_equal. now apply Hx. now apply IHForall. 
+Qed.
+
+Lemma on_snd_test_spec {A B} (P : B -> Prop) (p : B -> bool) (f g : B -> B) (x : A * B) :
+  P (snd x) -> (forall x, P x -> p x = true -> f x = g x) ->
+  test_snd p x = true ->
+  on_snd f x = on_snd g x.
+Proof.
+  intros. destruct x. unfold on_snd. simpl.
+  now rewrite H0; auto.
+Qed.
+
+Lemma map_def_test_spec (P : term -> Prop) p (f g : term -> term) (x : def term) :
+  P x.(dbody) -> P x.(dtype) -> (forall x, P x -> p x = true -> f x = g x) ->
+  test_def p x = true ->
+  map_def f x = map_def g x.
+Proof.
+  intros. destruct x. unfold map_def. simpl.
+  unfold test_def in H2; simpl in H2. rewrite andb_true_iff in H2.
+  rewrite !H1; intuition auto. 
+Qed.
+
+Lemma case_brs_forallb_map_spec {P : term -> Prop} {p : term -> bool}
+      {l} {f g : term -> term} :
+  tCaseBrsProp P (Forall P) l -> 
+  forallb (test_snd p) l = true ->
+  (forall x, P x -> p x = true -> f x = g x) ->
+  map (on_snd f) l = map (on_snd g) l.
+Proof.
+  intros.
+  eapply (forall_forallb_map_spec H H0).
+  intros.
+  eapply on_snd_test_spec; eauto.
+Qed.
+
+Lemma tfix_forallb_map_spec {P : term -> Prop} {p} {l} {f g : term -> term} :
+  tFixProp P (Forall P) l -> 
+  forallb (test_def p) l = true ->
+  (forall x, P x -> p x = true -> f x = g x) ->
+  map (map_def f) l = map (map_def g) l.
+Proof.
+  intros.
+  eapply (forall_forallb_map_spec H H0).
+  intros. destruct H2.
+  eapply map_def_test_spec; eauto.
+Qed.
+
 Ltac apply_spec :=
   match goal with
-    H : Forall _ _ |- map _ _ = map _ _ =>
+  | H : Forall _ _, H' : forallb _ _ = _ |- map _ _ = map _ _ =>
+    eapply (forall_forallb_map_spec H H')
+  | H : Forall _ _ |- map _ _ = map _ _ =>
     eapply (forall_map_spec H)
+  | H : tCaseBrsProp _ _ _, H' : forallb _ _ = _ |- map _ _ = map _ _ =>
+    eapply (case_brs_forallb_map_spec H H')
   | H : tCaseBrsProp _ _ _ |- map _ _ = map _ _ =>
     eapply (case_brs_map_spec H)
+  | H : tFixProp _ _ _, H' : forallb _ _ = _ |- map _ _ = map _ _ =>
+    eapply (tfix_forallb_map_spec H H')
   | H : tFixProp _ _ _ |- map _ _ = map _ _ =>
     eapply (tfix_map_spec H)
   end.
