theories/WeakSubst.v
@@ -1,0 +1,259 @@
+From Coq Require Import Bool String List Program BinPos Compare_dec Omega.
+From Template Require Import Template Ast Induction LiftSubst Typing.
+
+Set Asymmetric Patterns.
+Generalizable Variables Σ Γ t T.
+
+Definition app_context (Γ Γ' : context) : context := Γ' ++ Γ.
+Notation " Γ  ,,, Γ' " := (app_context Γ Γ') (at level 25, Γ' at next level, left associativity).
+Notation "#| Γ |" := (length Γ) (at level 0, format "#| Γ |").
+
+Lemma length_app_context Γ Γ' : #|Γ ,,, Γ'| = #|Γ| + #|Γ'|.
+Proof.
+  unfold app_context. rewrite app_length. omega.
+Qed.
+
+Definition map_decl (f : term -> term) (d : context_decl) : context_decl :=
+  {| decl_name := d.(decl_name);
+     decl_body := option_map f d.(decl_body);
+     decl_type := f d.(decl_type) |}.
+
+Definition lift_decl n k (d : context_decl) := map_decl (lift n k) d.
+
+Definition lift_context_rec n k (Γ : context) : nat * context :=
+  List.fold_right (fun decl '(k, Γ) => (S k, lift_decl n k decl :: Γ)) (k, []) Γ.
+
+Definition lift_context n k Γ := snd (lift_context_rec n k Γ).
+
+Lemma lift0_context k Γ : lift_context 0 k Γ = Γ.
+Proof.
+  unfold lift_context; induction Γ; simpl; trivial.
+  simpl. destruct lift_context_rec. simpl in *.
+  unfold lift_decl, map_decl. destruct a. simpl. rewrite IHΓ; f_equal.
+  rewrite lift_rec0. now destruct decl_body; simpl; rewrite ?lift_rec0.
+Qed.
+  
+Lemma lift_context_rec_fst n k Γ :
+  fst (lift_context_rec n k Γ) = #|Γ| + k.
+Proof.
+  induction Γ; simpl; auto.
+  destruct lift_context_rec; simpl in *.
+  congruence.
+Qed.
+Hint Rewrite lift_context_rec_fst : lift.
+
+Lemma lift_context_len n k Γ : #|lift_context n k Γ| = #|Γ|.
+Proof.
+  unfold lift_context; induction Γ; simpl; trivial.
+  destruct lift_context_rec. simpl in *. auto with arith.
+Qed.
+Hint Rewrite lift_context_len : lift.
+
+Lemma lift_context_snoc n k Γ d : lift_context n k (Γ ,, d) = lift_context n k Γ ,, lift_decl n (#|Γ| + k) d.
+Proof.
+  unfold lift_context.
+  simpl.
+  pose proof (lift_context_rec_fst n k Γ).
+  revert H. destruct lift_context_rec. simpl.
+  now intros ->.
+Qed.
+Hint Rewrite lift_context_snoc : lift.
+
+Lemma some_inj {A} {x y : A} : Some x = Some y -> x = y.
+Proof.
+  now intros [=].
+Qed.
+
+Lemma nth_error_app_ge v Γ Γ' : #|Γ'| <= v -> nth_error (Γ ,,, Γ') v = nth_error Γ (v - #|Γ'|).
+Proof.
+  revert v; induction Γ'; simpl; intros.
+
+  now rewrite Nat.sub_0_r.
+  destruct v. omega.
+  simpl. rewrite IHΓ'; easy.
+Qed.
+
+Lemma nth_error_app_lt v Γ Γ' : v < #|Γ'| -> nth_error (Γ ,,, Γ') v = nth_error Γ' v.
+Proof.
+  revert v; induction Γ'; simpl; intros. easy.
+
+  destruct v; trivial.
+  simpl. rewrite IHΓ'; easy.
+Qed.
+
+Lemma weaken_safe_nth_ge Γ Γ' v (isdecl : v < #|Γ ,,, Γ'|) Γ'' : #|Γ'| <= v ->
+  exists isdecl',
+  safe_nth (Γ ,,, Γ') (exist (fun n0 : nat => n0 < #|Γ ,,, Γ'|) v isdecl) =
+  safe_nth (Γ ,,, Γ'' ,,, lift_context #|Γ''| 0 Γ') (exist _ (#|Γ''| + v) isdecl').
+Proof.
+  simpl.
+  assert(#|Γ''| + v < #|Γ ,,, Γ'' ,,, lift_context #|Γ''| 0 Γ'|).
+  rewrite !length_app_context in *. autorewrite with lift. omega.
+  exists H.
+  apply some_inj; rewrite <- !nth_error_safe_nth.
+  rewrite nth_error_app_ge; try easy.
+  rewrite (nth_error_app_ge (_ + v)); rewrite ?lift_context_len; try easy.
+  rewrite nth_error_app_ge; rewrite ?lift_context_len; try easy.
+Qed.
+
+Lemma weaken_safe_nth_lt Γ Γ' v (isdecl : v < #|Γ ,,, Γ'|) Γ'' : v < #|Γ'| ->
+  exists isdecl',
+  safe_nth (Γ ,,, Γ'' ,,, lift_context #|Γ''| 0 Γ') (exist _ v isdecl') =
+  lift_decl #|Γ''| (#|Γ'| - S v)
+       (safe_nth (Γ ,,, Γ') (exist (fun n0 : nat => n0 < #|Γ ,,, Γ'|) v isdecl)).
+Proof.
+  simpl. intros Hv.
+  assert(v < #|Γ ,,, Γ'' ,,, lift_context #|Γ''| 0 Γ'|).
+  rewrite !length_app_context in *. autorewrite with lift. omega.
+  exists H.
+  apply some_inj. rewrite <- !nth_error_safe_nth.
+  rewrite nth_error_app_lt. 2:rewrite !length_app_context in H; autorewrite with lift; omega.
+  remember (safe_nth (Γ ,,, Γ') (exist _ v isdecl)) as nth.
+  apply (f_equal Some) in Heqnth. rewrite <- nth_error_safe_nth in Heqnth.
+  rewrite nth_error_app_lt in Heqnth; try easy.
+  clear isdecl H Γ.
+  revert Γ'' v Hv nth Heqnth.
+  induction Γ'; intros.
+  - easy.
+  - simpl. destruct v.
+    + simpl. unfold lift_context. simpl.
+      destruct lift_context_rec eqn:Heq.
+      pose proof (lift_context_rec_fst #|Γ''| 0 Γ'). rewrite Heq in H. simpl in H. subst n.
+      simpl. rewrite Nat.add_0_r, Nat.sub_0_r.
+      simpl in *. now injection Heqnth as ->.
+    + simpl.
+      unfold lift_context. simpl.
+      destruct lift_context_rec eqn:Heq.
+      pose proof (lift_context_rec_fst #|Γ''| 0 Γ'). rewrite Heq in H. simpl in H. subst n.
+      simpl in *.
+      assert (v < #|Γ'|) by easy.
+      specialize (IHΓ' Γ'' v  H nth Heqnth).
+      rewrite <- IHΓ'.
+      f_equal. unfold lift_context. rewrite Heq. reflexivity.
+Qed.  
+
+Lemma typecheck_closed Σ Γ t T :
+  type_global_env Σ -> type_local_env Σ Γ ->
+  Σ ;;; Γ |-- t : T -> closedn #|Γ| t && closedn #|Γ| T = true.
+Proof.
+  induction 3; simpl; rewrite ?andb_true_iff in *; try solve [intuition auto].
+  - elim (Nat.ltb_spec n #|Γ|); intuition.
+    admit (* Need induction with IHs for environments *).
+  - intuition auto.
+    + eapply IHtyping2. constructor; auto.
+      now exists s1. exact I.
+  - intuition; eapply IHtyping2; constructor; auto.
+    now exists s1. exact I.
+    now exists s1. exact I.
+  - intuition; try eapply IHtyping3; try constructor; auto.
+    now exists s1. now exists s1. 
+  - (* typing spine ind *) admit.
+  - admit.
+  - admit.
+  - admit.
+  - specialize (IHtyping H0).
+    intuition auto. admit. admit. admit. admit.
+  - (* proj *) admit.
+  - admit.
+  - admit.
+Admitted.
+
+Ltac forward H :=
+  match type of H with
+  | ?X -> ?Y => assert(x : X) ; [ | specialize (H x); clear x ]
+  end.
+
+Lemma weakening_rec Σ Γ Γ' Γ'' :
+  type_global_env Σ -> type_local_env Σ (Γ ,,, Γ') ->
+  type_local_env Σ (Γ ,,, Γ'' ,,, lift_context #|Γ''| 0 Γ') ->
+  `(Σ ;;; Γ ,,, Γ' |-- t : T ->
+    Σ ;;; Γ ,,, Γ'' ,,, lift_context #|Γ''| 0 Γ' |--
+    lift #|Γ''| #|Γ'| t : lift #|Γ''| #|Γ'| T).
+Proof.
+  intros HΣ HΓΓ' HΓ'' * H. revert Γ'' HΓ''. 
+  dependent induction H; intros Γ'' HΓ''; simpl in *; try solve [econstructor; eauto].
+
+  - elim (Nat.leb_spec); intros Hn.
+    + destruct (weaken_safe_nth_ge _ _ _ isdecl Γ'' Hn) as [isdecl' ->].
+      rewrite simpl_lift_rec; try omega. rewrite Nat.add_succ_r.
+      now constructor.
+    + destruct (weaken_safe_nth_lt _ _ _ isdecl Γ'' Hn) as [isdecl' H'].
+      apply (f_equal decl_type) in H'.
+      unfold lift_decl in H'. simpl in H'.
+      assert (forall t, lift0 (S n) (lift #|Γ''| (#|Γ'| - S n) t) = lift #|Γ''| #|Γ'| (lift0 (S n) t)).
+      intros. assert (#|Γ'| = S n + (#|Γ'| - S n)) by easy.
+      rewrite H at 2.
+      rewrite <- permute_lift_rec; try easy.
+      rewrite <- H. rewrite <- H'. constructor.
+
+  - econstructor; auto.
+    simpl.
+    specialize (IHtyping2 Γ (Γ' ,, vass n t) HΣ).
+    forward IHtyping2. constructor; simpl; auto. now exists s1.
+    specialize (IHtyping2 eq_refl Γ'').
+    forward IHtyping2. rewrite lift_context_snoc. constructor. simpl; auto.
+    exists s1. simpl. rewrite Nat.add_0_r. eapply IHtyping1; auto. exact I.
+    rewrite lift_context_snoc, plus_0_r in IHtyping2.
+    eapply IHtyping2.
+
+  - econstructor; auto.
+    simpl.
+    specialize (IHtyping2 Γ (Γ' ,, vass n t) HΣ).
+    forward IHtyping2. constructor; simpl; auto. now exists s1.
+    specialize (IHtyping2 eq_refl Γ'').
+    forward IHtyping2. rewrite lift_context_snoc. constructor. simpl; auto.
+    exists s1. simpl. rewrite Nat.add_0_r. eapply IHtyping1; auto. exact I.
+    rewrite lift_context_snoc, plus_0_r in IHtyping2.
+    eapply IHtyping2.
+
+
+  - econstructor; auto.
+    simpl.
+    specialize (IHtyping3 Γ (Γ' ,, vdef n b b_ty) HΣ).
+    forward IHtyping3. constructor; simpl; auto. now exists s1.
+    specialize (IHtyping3 eq_refl Γ'').
+    forward IHtyping3. rewrite lift_context_snoc, Nat.add_0_r.
+    constructor. simpl; auto.
+    exists s1. simpl. eapply IHtyping1; auto. simpl.
+    specialize (IHtyping2 Γ Γ' HΣ HΓΓ' eq_refl Γ'').
+    now eapply IHtyping2.
+    rewrite lift_context_snoc, plus_0_r in IHtyping3.
+    eapply IHtyping3.
+    
+
+  - econstructor; auto.
+    simpl.
+    admit.
+
+  - admit.
+  - admit.
+  - admit.
+
+  - admit.
+  - admit.
+  - admit.
+  - (* Conv *)
+    admit.
+Admitted.
+
+Lemma type_local_env_app Σ (Γ Γ' : context) : type_local_env Σ (Γ ,,, Γ') -> type_local_env Σ Γ.
+Admitted.
+
+Lemma weakening Σ Γ Γ' :
+  type_global_env Σ -> type_local_env Σ (Γ ,,, Γ') ->
+  `(Σ ;;; Γ |-- t : T ->
+    Σ ;;; Γ ,,, Γ' |-- lift0 #|Γ'| t : lift0 #|Γ'| T).
+Proof.
+  intros HΣ HΓΓ' * H.
+  pose (weakening_rec Σ Γ [] Γ').
+  forward t0; eauto.
+  forward t0; eauto. now eapply type_local_env_app in HΓΓ'. 
+Qed.
+
+Lemma substitution Σ Γ n u U :
+  type_global_env Σ -> type_local_env Σ Γ ->
+  `(Σ ;;; Γ ,, vass n U |-- t : T -> Σ ;;; Γ |-- u : U ->
+    Σ ;;; Γ |-- t {0 := u} : T {0 := u}).
+Proof.
+  intros HΣ HΓ * Ht Hu.
+Admitted.
